lowering/defs/bytecode/eval/evalCompilerBytecodeAbiExternalStaticScript.sml
@@ -14,7 +14,7 @@ val () = computeLib.upd_compset (computeLib.add_thms [i2w_pos])
 val () = Globals.max_print_depth := 20
 
 Theorem external_scalars_matches_python_oracle:
-  compile_vyper (K SOME) (o1_policy prague_capabilities)
+  compile_vyper (K SOME) (o1_policy all_capabilities)
     task090_external_scalars_program =
     SOME ^(evalCompilerBytecodeLib.read_hex_bytes "external_scalars.hex")
 Proof
@@ -22,7 +22,7 @@ Proof
 QED
 
 Theorem external_struct_matches_python_oracle:
-  compile_vyper (K SOME) (o1_policy prague_capabilities)
+  compile_vyper (K SOME) (o1_policy all_capabilities)
     task090_external_struct_program =
     SOME ^(evalCompilerBytecodeLib.read_hex_bytes "external_struct.hex")
 Proof
