lowering/defs/bytecode/eval/evalCompilerBytecodeScalarTypeBuiltinsScript.sml
@@ -25,14 +25,14 @@ val () = computeLib.upd_compset
           word_eq_scalar_decimal_hi_word])
 
 Theorem scalar_empty_matches_python_oracle:
-  compile_vyper (K SOME) (o1_policy prague_capabilities) scalar_empty_program =
+  compile_vyper (K SOME) (o1_policy all_capabilities) scalar_empty_program =
     SOME ^(evalCompilerBytecodeLib.read_hex_bytes "scalar_empty.hex")
 Proof
   EVAL_TAC
 QED
 
 Theorem scalar_decimal_bounds_matches_python_oracle:
-  compile_vyper (K SOME) (o1_policy prague_capabilities)
+  compile_vyper (K SOME) (o1_policy all_capabilities)
     scalar_decimal_bounds_program =
     SOME ^(evalCompilerBytecodeLib.read_hex_bytes "scalar_decimal_bounds.hex")
 Proof
@@ -40,7 +40,7 @@ Proof
 QED
 
 Theorem scalar_decimal_max_matches_python_oracle:
-  compile_vyper (K SOME) (o1_policy prague_capabilities)
+  compile_vyper (K SOME) (o1_policy all_capabilities)
     scalar_decimal_max_program =
     SOME ^(evalCompilerBytecodeLib.read_hex_bytes "scalar_decimal_max.hex")
 Proof
@@ -51,7 +51,7 @@ val () = computeLib.upd_compset
   (computeLib.add_thms [compileEnvTheory.type_bounds_def])
 
 Theorem scalar_integer_bounds_matches_python_oracle:
-  compile_vyper (K SOME) (o1_policy prague_capabilities)
+  compile_vyper (K SOME) (o1_policy all_capabilities)
     scalar_integer_bounds_program =
     SOME ^(evalCompilerBytecodeLib.read_hex_bytes "scalar_integer_bounds.hex")
 Proof
@@ -59,7 +59,7 @@ Proof
 QED
 
 Theorem scalar_integer_min_uint8_matches_python_oracle:
-  compile_vyper (K SOME) (o1_policy prague_capabilities)
+  compile_vyper (K SOME) (o1_policy all_capabilities)
     scalar_integer_min_uint8_program =
     SOME ^(evalCompilerBytecodeLib.read_hex_bytes "scalar_integer_min_uint8.hex")
 Proof
@@ -67,7 +67,7 @@ Proof
 QED
 
 Theorem scalar_integer_max_int256_matches_python_oracle:
-  compile_vyper (K SOME) (o1_policy prague_capabilities)
+  compile_vyper (K SOME) (o1_policy all_capabilities)
     scalar_integer_max_int256_program =
     SOME ^(evalCompilerBytecodeLib.read_hex_bytes "scalar_integer_max_int256.hex")
 Proof
@@ -78,7 +78,7 @@ val () = computeLib.upd_compset
   (computeLib.add_thms [compileEnvTheory.type_bounds_def])
 
 Theorem scalar_convert_integer_matches_python_oracle:
-  compile_vyper (K SOME) (o1_policy prague_capabilities)
+  compile_vyper (K SOME) (o1_policy all_capabilities)
     scalar_convert_integer_program =
     SOME ^(evalCompilerBytecodeLib.read_hex_bytes "scalar_convert_integer.hex")
 Proof
@@ -86,7 +86,7 @@ Proof
 QED
 
 Theorem scalar_convert_address_matches_python_oracle:
-  compile_vyper (K SOME) (o1_policy prague_capabilities)
+  compile_vyper (K SOME) (o1_policy all_capabilities)
     scalar_convert_address_program =
     SOME ^(evalCompilerBytecodeLib.read_hex_bytes "scalar_convert_address.hex")
 Proof
@@ -94,7 +94,7 @@ Proof
 QED
 
 Theorem scalar_convert_bytes_fixed_matches_python_oracle:
-  compile_vyper (K SOME) (o1_policy prague_capabilities)
+  compile_vyper (K SOME) (o1_policy all_capabilities)
     scalar_convert_bytes_fixed_program =
     SOME ^(evalCompilerBytecodeLib.read_hex_bytes "scalar_convert_bytes_fixed.hex")
 Proof
@@ -102,7 +102,7 @@ Proof
 QED
 
 Theorem scalar_convert_uint_to_bytes32_matches_python_oracle:
-  compile_vyper (K SOME) (o1_policy prague_capabilities)
+  compile_vyper (K SOME) (o1_policy all_capabilities)
     scalar_convert_uint_to_bytes32_program =
     SOME ^(evalCompilerBytecodeLib.read_hex_bytes "scalar_convert_uint_to_bytes32.hex")
 Proof
@@ -110,7 +110,7 @@ Proof
 QED
 
 Theorem scalar_convert_bytes32_to_address_matches_python_oracle:
-  compile_vyper (K SOME) (o1_policy prague_capabilities)
+  compile_vyper (K SOME) (o1_policy all_capabilities)
     scalar_convert_bytes32_to_address_program =
     SOME ^(evalCompilerBytecodeLib.read_hex_bytes "scalar_convert_bytes32_to_address.hex")
 Proof
@@ -118,7 +118,7 @@ Proof
 QED
 
 Theorem scalar_convert_bytes32_to_bytes4_matches_python_oracle:
-  compile_vyper (K SOME) (o1_policy prague_capabilities)
+  compile_vyper (K SOME) (o1_policy all_capabilities)
     scalar_convert_bytes32_to_bytes4_program =
     SOME ^(evalCompilerBytecodeLib.read_hex_bytes "scalar_convert_bytes32_to_bytes4.hex")
 Proof
@@ -126,7 +126,7 @@ Proof
 QED
 
 Theorem scalar_convert_bytes_dynamic_matches_python_oracle:
-  compile_vyper (K SOME) (o1_policy prague_capabilities)
+  compile_vyper (K SOME) (o1_policy all_capabilities)
     scalar_convert_bytes_dynamic_program =
     SOME ^(evalCompilerBytecodeLib.read_hex_bytes "scalar_convert_bytes_dynamic.hex")
 Proof
