lowering/defs/bytecode/eval/evalCompilerBytecodeStateScript.sml
@@ -16,7 +16,7 @@ val () = computeLib.upd_compset (computeLib.add_thms [i2w_pos])
 val () = Globals.max_print_depth := 20
 
 Theorem storage_scalar_loop_matches_python_oracle:
-  compile_vyper (K SOME) (o1_policy prague_capabilities)
+  compile_vyper (K SOME) (o1_policy all_capabilities)
     storage_scalar_loop_program =
     SOME ^(evalCompilerBytecodeLib.read_hex_bytes "storage_scalar_loop.hex")
 Proof
@@ -24,7 +24,7 @@ Proof
 QED
 
 Theorem storage_array_matches_python_oracle:
-  compile_vyper (K SOME) (o1_policy prague_capabilities)
+  compile_vyper (K SOME) (o1_policy all_capabilities)
     storage_array_program =
     SOME ^(evalCompilerBytecodeLib.read_hex_bytes "storage_array.hex")
 Proof
@@ -32,7 +32,7 @@ Proof
 QED
 
 Theorem storage_dynarray_matches_python_oracle:
-  compile_vyper (K SOME) (o1_policy prague_capabilities)
+  compile_vyper (K SOME) (o1_policy all_capabilities)
     storage_dynarray_program =
     SOME ^(evalCompilerBytecodeLib.read_hex_bytes "storage_dynarray.hex")
 Proof
@@ -40,7 +40,7 @@ Proof
 QED
 
 Theorem storage_mapping_matches_python_oracle:
-  compile_vyper (K SOME) (o1_policy prague_capabilities)
+  compile_vyper (K SOME) (o1_policy all_capabilities)
     storage_mapping_program =
     SOME ^(evalCompilerBytecodeLib.read_hex_bytes "storage_mapping.hex")
 Proof
@@ -48,7 +48,7 @@ Proof
 QED
 
 Theorem storage_struct_matches_python_oracle:
-  compile_vyper (K SOME) (o1_policy prague_capabilities)
+  compile_vyper (K SOME) (o1_policy all_capabilities)
     storage_struct_program =
     SOME ^(evalCompilerBytecodeLib.read_hex_bytes "storage_struct.hex")
 Proof
@@ -56,7 +56,7 @@ Proof
 QED
 
 Theorem transient_scalar_matches_python_oracle:
-  compile_vyper (K SOME) (o1_policy prague_capabilities)
+  compile_vyper (K SOME) (o1_policy all_capabilities)
     transient_scalar_program =
     SOME ^(evalCompilerBytecodeLib.read_hex_bytes "transient_scalar.hex")
 Proof
